Utlc/Examples.v
@@ -1,0 +1,20 @@
+Require Import Nat.
+Require Import List.
+Require Import UTLC.LC.
+Require Import UTLC.Alpha_eq.
+
+
+Definition Id : LC :=  Abs (Var 1).
+
+Definition K : LC := Abs (Abs (Var 2)).
+
+Definition K' : LC := Abs (Abs (Var 1)).
+
+Definition S : LC := Abs (Abs (Abs (App ((App (Var 3 , Var 1)), (App (Var 2 , Var 1)))))).
+
+Definition ω : LC := Abs (App (Var 1, Var 1)).
+
+Definition Ω : LC := App (ω, ω). 
+
+Definition Y : LC := Abs (App (Abs (App ( Var 2, App (Var 1, Var 1))) , Abs (App ( Var 2, App (Var 1, Var 1))))).
+
